Pcc116Code/Aula13.lean
@@ -2,4 +2,141 @@
 
 import Mathlib.Data.Nat.Defs 
 
+-- representing De Bruijn indexes 
 
+inductive Idx {A : Type}(x : A) : List A → Type where 
+| Here : ∀ {xs}, Idx x (x :: xs)
+| There : ∀ {ys y}, Idx x ys → Idx x (y :: ys)
+
+def index {A : Type}{x : A}{xs} : Idx x xs → ℕ 
+| Idx.Here => 0
+| Idx.There idx => (index idx) + 1
+
+inductive Lookup {A : Type}(xs : List A) : ℕ → Type where 
+| Inside : ∀ (x : A)(p : Idx x xs), Lookup xs (index p)
+| Outside : ∀ (m : ℕ), Lookup xs (m + List.length xs)
+
+def lookup {A : Type} : (xs : List A) → (n : ℕ) → Lookup xs n 
+| [] , n => Lookup.Outside n
+| x :: _, 0 => Lookup.Inside x Idx.Here 
+| _ :: xs, n + 1 => 
+  match lookup xs n with 
+  | Lookup.Inside y idx => Lookup.Inside y (Idx.There idx)
+  | Lookup.Outside m => Lookup.Outside m  
+
+-- type syntax 
+
+inductive Ty : Type where 
+| Base : Ty 
+| Arr : Ty → Ty → Ty 
+deriving Repr 
+
+def eqTy (t t' : Ty) : Decidable (t = t') := 
+  match t, t' with 
+  | Ty.Base, Ty.Base => Decidable.isTrue rfl 
+  | Ty.Arr t1 t2, Ty.Arr t1' t2' => 
+    match eqTy t1 t1', eqTy t2 t2' with 
+    | Decidable.isTrue rfl, Decidable.isTrue rfl => Decidable.isTrue rfl 
+    | Decidable.isTrue p , Decidable.isFalse q => by 
+      apply Decidable.isFalse 
+      intro H 
+      cases H 
+      simp at * 
+    | Decidable.isFalse p, Decidable.isTrue q => by 
+      apply Decidable.isFalse 
+      intro H
+      cases H 
+      simp at * 
+    | Decidable.isFalse p, Decidable.isFalse q => by 
+      apply Decidable.isFalse 
+      intro H 
+      cases H 
+      simp at * 
+  | Ty.Base, Ty.Arr _ _ => by 
+    apply Decidable.isFalse 
+    intro H
+    cases H 
+  | Ty.Arr _ _, Ty.Base => by 
+    apply Decidable.isFalse 
+    intro H ; cases H 
+
+instance : DecidableEq Ty := eqTy  
+
+-- definition of untyped syntax 
+
+inductive Raw : Type where 
+| UVar : ℕ → Raw 
+| UApp : Raw → Raw → Raw 
+| ULam : Ty → Raw → Raw 
+deriving Repr 
+
+-- typed syntax 
+
+abbrev Ctx := List Ty 
+
+inductive Term : Ctx → Ty → Type where 
+| TVar : ∀ {ctx t}, Idx t ctx → Term ctx t 
+| TApp : ∀ {ctx t t'}, Term ctx (Ty.Arr t t') → 
+                       Term ctx t → 
+                       Term ctx t' 
+| TLam : ∀ {ctx t'} t, Term (t :: ctx) t' → 
+                       Term ctx (Ty.Arr t t')
+
+def erase {ctx t} : Term ctx t → Raw 
+| Term.TVar idx => Raw.UVar (index idx)
+| Term.TApp t1 t2 => Raw.UApp (erase t1) (erase t2)
+| Term.TLam t t1 => Raw.ULam t (erase t1)
+
+-- certified type checker 
+
+inductive Check (ctx : Ctx) : Raw → Type where 
+| Ok : ∀ (t : Ty)(e : Term ctx t), Check ctx (erase e)
+| Bad : ∀ {e : Raw}, Check ctx e
+
+def check : ∀ (ctx : Ctx)(e : Raw), Check ctx e
+| ctx, Raw.UVar n => 
+    match lookup ctx n with 
+    | Lookup.Inside t idx => Check.Ok t (Term.TVar idx)
+    | Lookup.Outside _ => Check.Bad 
+| ctx, Raw.UApp e1 e2 => 
+    match check ctx e1, check ctx e2 with 
+    | Check.Ok Ty.Base _ , _ => Check.Bad 
+    | Check.Ok (Ty.Arr t1 t2) tm1, Check.Ok t1' tm2 =>  
+      match decEq t1 t1' with 
+      | .isTrue p => by 
+        cases p 
+        exact (Check.Ok t2 (Term.TApp tm1 tm2))
+      | .isFalse _ => Check.Bad 
+    | _, _ => Check.Bad
+| ctx, Raw.ULam t e1 => 
+    match check (t :: ctx) e1 with 
+    | Check.Ok t' tm1 => Check.Ok _ (Term.TLam t tm1)
+    | Check.Bad => Check.Bad 
+
+-- defining the semantics by embedding it into Lean 
+
+-- 1. interpreting types 
+
+def Ty.asType : Ty → Type 
+| Ty.Base => Bool 
+| Ty.Arr t1 t2 => t1.asType -> t2.asType 
+
+-- 2. intepreting environments 
+
+@[reducible]
+def semEnv : Ctx → Type 
+| [] => Unit 
+| x :: xs => x.asType × semEnv xs 
+
+-- 3. interpreting indexes 
+
+def semIdx {ctx t} : Idx t ctx → semEnv ctx → t.asType 
+| Idx.Here, (v, _) => v
+| Idx.There idx, (_, env) => semIdx idx env
+
+-- 4. interpreting terms 
+
+def interp {ctx t} : Term ctx t → semEnv ctx → t.asType 
+| Term.TVar idx, env => semIdx idx env 
+| Term.TApp t1 t2, env => (interp t1 env) (interp t2 env)
+| Term.TLam _ t, env => λ v => interp t (v, env) 
